make aes more uniform

code/aes/vec128.h
@@ -16,13 +16,32 @@ typedef __m128i Lib_Vec128_vec128;
 #define Lib_Vec128_ni_aes_keygen_assist(x0, x1) \
   (_mm_aeskeygenassist_si128(x0, x1))
 
+#define Lib_Vec128_ni_clmul(x0, x1, x2)		\
+  (_mm_clmulepi64_si128(x0, x1, x2))
+
+
+
+
 #define Lib_Vec128_vec128_xor(x0, x1) \
   (_mm_xor_si128(x0, x1))
 
-#define Lib_Vec128_vec128_shift_left(x0, x1) \
-  (_mm_slli_si128(x0, x1/8))
+#define Lib_Vec128_vec128_or(x0, x1) \
+  (_mm_or_si128(x0, x1))
 
-#define Lib_Vec128_vec128_shuffle32(x0, x1) \
+#define Lib_Vec128_vec128_shift_left(x0, x1) \
+  (_mm_slli_si128(x0, (x1)/8))
+
+#define Lib_Vec128_vec128_shift_right(x0, x1) \
+  (_mm_srli_si128(x0, (x1)/8))
+
+#define Lib_Vec128_vec128_shift_left64(x0, x1) \
+  (_mm_slli_epi64(x0, x1))
+
+#define Lib_Vec128_vec128_shift_right64(x0, x1) \
+  (_mm_srli_epi64(x0, x1))
+
+
+#define Lib_Vec128_vec128_shuffle32(x0, x1)	\
   (_mm_shuffle_epi32(x0, x1))
 
 #define Lib_Vec128_vec128_shuffle32_spec(x0, x1, x2, x3) \
@@ -34,7 +53,13 @@ typedef __m128i Lib_Vec128_vec128;
 #define Lib_Vec128_vec128_store_le(x0, x1) \
   (_mm_storeu_si128((__m128i*)(x0), x1))
 
-#define Lib_Vec128_vec128_insert32(x0, x1, x2) \
+#define Lib_Vec128_vec128_load_be(x0)		\
+  (_mm_shuffle_epi8(_mm_loadu_si128((__m128i*)(x0)), _mm_set_epi8(0, 1, 2, 3, 4, 5, 6, 7, 8, 9, 10, 11, 12, 13, 14, 15)))
+
+#define Lib_Vec128_vec128_store_be(x0, x1)	\
+  (_mm_storeu_si128((__m128i*)(x0), _mm_shuffle_epi8(x1, _mm_set_epi8(0, 1, 2, 3, 4, 5, 6, 7, 8, 9, 10, 11, 12, 13, 14, 15))))
+
+#define Lib_Vec128_vec128_insert32(x0, x1, x2)	\
   (_mm_insert_epi32(x0, x1, x2))
 
 #define Lib_Vec128_vec128_zero  \
